wip adding support for 8bit MMIO
[does not compile yet]

investigations/bedrock2/LibBase/MMIOLabels.v
@@ -1,11 +1,44 @@
 (* names for the MMIO load/store events to record in the I/O trace *)
 
 Require Import Coq.Strings.String. Local Open Scope string_scope.
+Require Import bedrock2.Syntax.
 
-Definition READ8 := "READ8".
-Definition READ16 := "READ16".
-Definition READ32 := "READ32".
+Definition READ_PREFIX := "READ".
+Definition READ8 := READ_PREFIX ++ "8".
+Definition READ16 := READ_PREFIX ++ "16".
+Definition READ32 := READ_PREFIX ++ "32".
+Definition READW := READ_PREFIX ++ "W". (* read 32 or 64 bits depending on bitwidth of machine *)
 
-Definition WRITE8 := "WRITE8".
-Definition WRITE16 := "WRITE16".
-Definition WRITE32 := "WRITE32".
+Definition WRITE_PREFIX := "WRITE".
+Definition WRITE8 := WRITE_PREFIX ++ "8".
+Definition WRITE16 := WRITE_PREFIX ++ "16".
+Definition WRITE32 := WRITE_PREFIX ++ "32".
+Definition WRITEW := WRITE_PREFIX ++ "W". (* write 32 or 64 bits depending on bitwidth of machine *)
+
+Definition access_size_to_MMIO_suffix(sz: access_size): string :=
+  match sz with
+  | access_size.one => "8"
+  | access_size.two => "16"
+  | access_size.four => "32"
+  | access_size.word => "W"
+  end.
+
+Definition access_size_to_MMIO_read(sz: access_size): string :=
+  READ_PREFIX ++ access_size_to_MMIO_suffix sz.
+
+Definition access_size_to_MMIO_write(sz: access_size): string :=
+  WRITE_PREFIX ++ access_size_to_MMIO_suffix sz.
+
+Lemma access_size_to_MMIO_read_inj: forall sz1 sz2,
+    access_size_to_MMIO_read sz1 = access_size_to_MMIO_read sz2 ->
+    sz1 = sz2.
+Proof.
+  destruct sz1; destruct sz2; cbv; congruence.
+Qed.
+
+Lemma access_size_to_MMIO_write_inj: forall sz1 sz2,
+    access_size_to_MMIO_write sz1 = access_size_to_MMIO_write sz2 ->
+    sz1 = sz2.
+Proof.
+  destruct sz1; destruct sz2; cbv; congruence.
+Qed.
